Tests/STLC_Eval/TrmDemo.lean
@@ -1,0 +1,59 @@
+import «Tests».STLC_Eval.ValDemo
+
+namespace Tests.STLC_Eval.Sanity
+
+open Lp2lc.Active.Util
+open Lp2lc.Active.STLC
+open Tests.STLC_Eval.Sanity.Symbolic
+
+namespace Trm
+
+def vFalse : Trm :=
+  .val Val.vFalse
+
+def vTrue : Trm :=
+  .val Val.vTrue
+
+def primitiveIdFn : Trm :=
+  .val Val.idFn
+
+def primitiveIdFnOnFalse : Trm :=
+  .apply primitiveIdFn vFalse
+
+def primitiveTrueFn : Trm :=
+  .val (.fn (fun _ref => vTrue) .primitive)
+
+def primitiveTrueFnOnFalse : Trm :=
+  .apply primitiveTrueFn vFalse
+
+def get1st : Trm :=
+  .val
+    (.fn (fun firstRef =>
+      .val (.fn (fun _secondRef => .ref firstRef) .primitive))
+      .primitive)
+
+def get1stOnTuple : Trm :=
+  .apply (.apply get1st vFalse) vTrue
+
+namespace Malformed
+
+def primitiveApply : Trm :=
+  .apply vFalse vTrue
+
+def bodyFails : Trm :=
+  .val (.fn (fun _ref => primitiveApply) .primitive)
+
+def bodyFailsOnFalse : Trm :=
+  .apply bodyFails vFalse
+
+def idFnOnPrimitiveApply : Trm :=
+  .apply primitiveIdFn primitiveApply
+
+def primitiveApplyOnFalse : Trm :=
+  .apply primitiveApply vFalse
+
+end Malformed
+
+end Trm
+
+end Sanity
