Tests/STLC_Eval/TrmSpec.lean
@@ -1,0 +1,72 @@
+import «Tests».STLC_Eval.Fixture
+
+namespace Tests.STLC_Eval.Sanity
+
+namespace Trm
+
+open Lp2lc.Active.Util
+open Lp2lc.Active.STLC
+open Tests.STLC_Eval.Sanity.Symbolic
+
+section eval
+
+variable [env : @RuntimeEnv Symbolic.I]
+
+example : (vFalse : Trm).eval 0 = .outOfFuel := rfl
+
+example : (vFalse : Trm).eval.shouldYields Val.vFalse := by
+  constructor
+  · exact ⟨1, rfl⟩
+  · rfl
+
+example :
+    let ref := env.valueRefs.save ⟨Val.vFalse, env.canEvalAny Val.vFalse⟩
+    (AST.Trm.ref ref).eval 1 = .yield (some Val.vFalse) := by
+  simp [AST.Trm.eval]
+
+example : (primitiveIdFnOnFalse : Trm).eval 1 = .outOfFuel := rfl
+
+example : (primitiveIdFnOnFalse : Trm).eval.shouldYields Val.vFalse := by
+  constructor
+  · exact ⟨2, by simp [AST.Trm.eval, primitiveIdFnOnFalse, primitiveIdFn, vFalse, Val.idFn]⟩
+  · rfl
+
+example : (primitiveTrueFnOnFalse : Trm).eval.shouldYields Val.vTrue := by
+  constructor
+  · exact ⟨2, rfl⟩
+  · rfl
+
+example : (get1stOnTuple : Trm).eval.shouldYields Val.vFalse := by
+  constructor
+  · exact ⟨3, by simp [AST.Trm.eval, get1stOnTuple, get1st, vFalse, vTrue]⟩
+  · rfl
+
+example : (.apply primitiveIdFnOnFalse vTrue : Trm).eval 2 = .outOfFuel := rfl
+
+example : (.apply primitiveIdFn primitiveIdFnOnFalse : Trm).eval 2 = .outOfFuel := rfl
+
+example : (Malformed.primitiveApply : Trm).eval.shouldFail := by
+  constructor
+  · exact ⟨2, rfl⟩
+  · rfl
+
+example : (Malformed.bodyFailsOnFalse : Trm).eval.shouldFail := by
+  constructor
+  · exact ⟨3, rfl⟩
+  · rfl
+
+example : (Malformed.idFnOnPrimitiveApply : Trm).eval.shouldFail := by
+  constructor
+  · exact ⟨3, rfl⟩
+  · rfl
+
+example : (Malformed.primitiveApplyOnFalse : Trm).eval.shouldFail := by
+  constructor
+  · exact ⟨3, rfl⟩
+  · rfl
+
+end eval
+
+end Trm
+
+end Sanity
