Tests/STLC_Eval/ValDemo.lean
@@ -1,0 +1,37 @@
+import «Lp2lc».Active.STLC.STLCDef
+
+namespace Tests.STLC_Eval.Sanity
+
+open Lp2lc.Active.Util
+open Lp2lc.Active.STLC
+
+inductive Symbol
+
+namespace Symbolic
+
+@[reducible] def I : Free where
+  Index := Symbol
+  Data := String
+
+abbrev Typ := AST.Typ I
+abbrev Val := AST.Val I
+abbrev Trm := AST.Trm I
+
+end Symbolic
+
+open Symbolic
+
+namespace Val
+
+def vFalse : Val :=
+  .primitive "false"
+
+def vTrue : Val :=
+  .primitive "true"
+
+def idFn : Val :=
+  .fn (fun ref => .ref ref) .primitive
+
+end Val
+
+end Sanity
