Tests/package.lean
@@ -5,3 +5,4 @@ import «Tests».PrimeRefinementDemo
 import «Tests».DOT.Sanity
 import «Tests».DTLC.package
 import «Tests».STLC.package
+import «Tests».STLC_Eval.package
